Include ghost name in dh_auth spec.

dh_auth.v
@@ -10,12 +10,22 @@ Set Implicit Arguments.
 Unset Strict Implicit.
 Unset Printing Implicit Defensive.
 
+(* MOVE *)
+Lemma lc_fupd_elim_later_pers `{invGS Σ} E (P : iProp Σ) :
+  £ 1 -∗ □ ▷ P ={E}=∗ □ P.
+Proof.
+rewrite bi.later_intuitionistically_2.
+exact: lc_fupd_elim_later.
+Qed.
+
 Section Verif.
 
 Context `{!heapGS Σ, !cryptisGS Σ, !sessionGS Σ}.
 Notation iProp := (iProp Σ).
 
 Implicit Types (rl : role) (t kI kR nI nR sI sR kS : term).
+Implicit Types (γ γa γb : gname) (ok : bool).
+Implicit Types (ts : nat) (T : gset term).
 
 Variable N : namespace.
 
@@ -75,48 +85,57 @@ Definition responder : val := λ: "c" "vkR" "skR",
   let: "gab" := texp "ga" "b" in
   SOME ("vkI", "gab").
 
-Definition in_honest kI kR (T : gset term) : bool :=
+Definition in_honest kI kR T : bool :=
   bool_decide (TKey Enc kI ∈ T ∧ TKey Enc kR ∈ T).
 
 Definition dh_auth_pred t : iProp :=
-  ⌜∀ g ts, t = TExp g ts → length ts = 1⌝.
+  ⌜∀ g ks, t = TExp g ks → length ks = 1⌝.
 
 Definition msg2_pred kR m2 : iProp :=
-  ∃ ga b kI n T,
+  ∃ ga b kI n T γb,
     ⌜m2 = Spec.of_list [ga; TExp (TInt 0) [b]; TKey Dec kI]⌝ ∗
-    (public b ↔ ▷ □ (compromised_at n (TKey Enc kR) ∨
-                     compromised_at n (TKey Enc kI))) ∗
+    (public b ↔ ▷ □ (compromised_at n (TKey Enc kI) ∨
+                     compromised_at n (TKey Enc kR))) ∗
     (∀ t, dh_pred b t ↔ ▷ □ dh_auth_pred t) ∗
     ◯H{n} T ∗
-    nonce_meta b (N.@"session") (Resp, ga, b, kI, kR, n, T).
+    nonce_meta b (N.@"session") (Resp, ga, kI, kR, n, T, γb).
 
 Definition msg3_pred kI m3 : iProp :=
-  ∃ a gb kR n T,
+  ∃ a gb kR n T γa,
     ⌜m3 = Spec.of_list [TExp (TInt 0) [a]; gb; TKey Dec kR]⌝ ∗
-    (public a ↔ ▷ □ ⌜TKey Enc kI ∉ T ∨ TKey Enc kR ∉ T⌝) ∗
+    (public a ↔ ▷ □ ⌜negb (in_honest kI kR T)⌝) ∗
     (∀ t, dh_pred a t ↔ ▷ □ dh_auth_pred t) ∗
     ◯H{n} T ∗
-    nonce_meta a (N.@"session") (Init, gb, a, kI, kR, n, T) ∗
+    nonce_meta a (N.@"session") (Init, gb, kI, kR, n, T, γa) ∗
     (public (TKey Enc kR) ∨
-     ∃ b n' (T' : gset term),
+     ∃ b n' T' γb,
        ⌜gb = TExp (TInt 0) [b]⌝ ∗
        ⌜n' ≤ n⌝ ∗
-       nonce_meta b (N.@"session") (Resp, TExp (TInt 0) [a], b, kI, kR, n', T')).
+       nonce_meta b (N.@"session")
+         (Resp, TExp (TInt 0) [a], kI, kR, n', T', γb)).
 
 Definition dh_auth_ctx : iProp :=
   enc_pred (N.@"m2") msg2_pred ∗
   enc_pred (N.@"m3") msg3_pred.
 
-Definition session kI kR k rl : iProp :=
+Definition session γ kI kR k rl ok : iProp :=
   ∃ share x ts T,
     ⌜k = Spec.texp share x⌝ ∗
+    ⌜ok = in_honest kI kR T⌝ ∗
     ◯H{ts} T ∗
-    nonce_meta x (N.@"session") (rl, share, x, kI, kR, ts, T).
+    nonce_meta x (N.@"session") (rl, share, kI, kR, ts, T, γ) ∗
+    if ok then ∃ y ts' T' γ',
+        ⌜share = TExp (TInt 0) [y]⌝ ∗
+        ⌜ts' ≤ ts⌝ ∗
+        nonce_meta y (N.@"session")
+          (swap_role rl, TExp (TInt 0) [x], kI, kR, ts', T', γ')
+    else
+      True.
 
 Ltac protocol_failure :=
   by intros; wp_pures; iApply ("Hpost" $! None); iFrame.
 
-Lemma wp_initiator c kI kR dq n T E :
+Lemma wp_initiator c kI kR dq n T γ E :
   ↑cryptisN ⊆ E →
   ↑N ⊆ E →
   channel c -∗
@@ -130,18 +149,15 @@ Lemma wp_initiator c kI kR dq n T E :
       ●H{dq|n} T ∗
       if okS is Some kS then
         minted kS ∗
-        session kI kR kS Init ∗
-        if in_honest kI kR T then
-          session kI kR kS Resp ∗
-          □ (public kS -∗ ▷ False)
-        else public kS
+        session γ kI kR kS Init (in_honest kI kR T) ∗
+        □ (public kS ↔ ▷ ⌜negb (in_honest kI kR T)⌝)
       else True
  }}}.
 Proof.
-rewrite /initiator /in_honest bool_decide_decide.
+rewrite /initiator.
 iIntros (??) "#chan_c #ctx #(? & ?) #p_kI #p_kR %Ψ !> hon Hpost".
 wp_pures. wp_bind (mknonce _).
-iApply (wp_mknonce (λ _, ⌜TKey Enc kI ∉ T ∨ TKey Enc kR ∉ T⌝)%I
+iApply (wp_mknonce (λ _, ⌜negb (in_honest kI kR T)⌝)%I
           dh_auth_pred).
 iIntros "%a #m_a #p_a #a_pred token".
 iPoseProof (honest_auth_frag with "hon") as "#honI".
@@ -153,12 +169,13 @@ iAssert (public (TExp (TInt 0) [a])) as "p_ga".
 { iApply public_TExp1.
   rewrite minted_TInt. do 2![iSplit => //].
   iRight. iApply "a_pred". iModIntro. iModIntro.
-  iIntros "%g %ts %e".
+  iIntros "%g %ks %e".
   case/TExp_inj: e => _ perm.
   by rewrite -(Permutation_length perm). }
 wp_bind (send _ _). iApply wp_send => //.
 { rewrite public_of_list /=. iModIntro.
   do 2?[iSplit => //]. }
+wp_pure _ credit:"H3".
 wp_pures. wp_bind (recv _). iApply wp_recv => //.
 iIntros "%m2 #p_m2". wp_tdec m2; last by protocol_failure.
 wp_pures. wp_list_of_term m2; last by protocol_failure.
@@ -178,76 +195,102 @@ rewrite minted_TEnc minted_tag minted_of_list /=.
 iDestruct "m_m2" as "(_ & _ & m_gb & _)".
 wp_pures. wp_bind (texp _ _). iApply wp_texp.
 wp_pures. wp_list. wp_term_of_list. wp_tenc.
-iMod (term_meta_set _ _ (Init, gb, a, kI, kR, n, T)
+iMod (term_meta_set _ _ (Init, gb, kI, kR, n, T, γ)
        (N.@"session") with "token") as "#sessionI" => //.
-iAssert (
-    ▷ (public (TKey Enc kR) ∨
-    ∃ b n' (T' : gset term),
+iAssert ( |={E}=>
+    ●H{dq|n} T ∗
+    (compromised_at n (TKey Enc kR) ∨
+    ∃ b n' T' γ',
      ⌜gb = TExp (TInt 0) [b]⌝ ∗
      ⌜n' ≤ n⌝ ∗
-     nonce_meta b (N.@"session") (Resp, TExp (TInt 0) [a], b, kI, kR, n', T')))%I
-  as "#p_m2'".
+     □ (public b ↔ ▷ □ (compromised_at n' (TKey Enc kI) ∨
+                        compromised_at n' (TKey Enc kR))) ∗
+     nonce_meta b (N.@"session")
+       (Resp, TExp (TInt 0) [a], kI, kR, n', T', γ')))%I
+  with "[hon H3]"
+  as "{p_m2} > [hon #p_m2]".
 { iPoseProof (public_TEncE with "p_m2 [//]") as "{p_m2} p_m2".
-  iDestruct "p_m2" as "[[? _]  | (#i_m2 & _ & _)]"; first by eauto.
-  iModIntro. iRight.
+  iDestruct "p_m2" as "[[comp _]  | (#i_m2 & _ & _)]".
+  { iMod (compromised_atI with "[ctx] [H3] [hon] [comp]")
+      as "[hon comp']" => //; try solve_ndisj. }
+  iMod (lc_fupd_elim_later_pers with "H3 i_m2") as "{i_m2} #i_m2".
   iDestruct "i_m2"
-    as "(%ga & %b & %kI' & %n' & %T' & %e_m2 & _ & _ & honR & pred_b)".
+    as "(%ga & %b & %kI' & %n' & %T' & %γr & %e_m2 & ? & _ & honR & pred_b)".
   case/Spec.of_list_inj: e_m2 => <- -> <- {ga gb kI'}.
-  iPoseProof (honest_auth_frag_agree with "hon honR") as "[%n'_n _]".
-  iExists _, _, _. iSplit => //. iSplit; last by [].
+  iPoseProof (honest_auth_frag_agree with "hon honR") as "[% %]".
+  iModIntro. iFrame. iRight.
+  iExists _, _, _, _. iSplit => //. iSplit => //. iSplit; last by [].
   by []. }
 wp_pures. wp_bind (send _ _). iApply wp_send => //.
 { iModIntro.
   iApply public_TEncIS => //.
   - by rewrite !public_minted !minted_TKey.
-  - iModIntro. iExists a, gb, kR, n, T. by do ![iSplitL => //].
+  - iModIntro. iExists a, gb, kR, n, T, γ. do ![iSplitL => //].
+    iDestruct "p_m2" as "[?|p_m2]".
+    { iLeft. by iApply compromised_at_public. }
+    iDestruct "p_m2" as "(%b & %n' & %T' & %γ' & % & % & ? & ?)".
+    iRight. iExists b, n', T', γ'. by eauto.
   - rewrite minted_of_list /= minted_TExp /= minted_TInt minted_TKey.
     rewrite !public_minted !minted_TKey. by do ![iSplitL => //].
   - iIntros "!> _".
     rewrite public_of_list /=.
     by do ![iSplit => //]. }
-iAssert (session kI kR (Spec.texp gb a) Init) as "#sessionI'".
-{ iExists gb, a, n, T; eauto. }
-case: decide => [[honI honR]|cor]; last first.
-{ iAssert (public (Spec.texp gb a)) as "#p_kS".
-  iApply public_texp => //.
-  iApply "p_a". by rewrite not_and_r in cor.
+iAssert (session γ kI kR (Spec.texp gb a) Init (in_honest kI kR T))
+  as "#sessionI'".
+{ iExists gb, a, n, T.
+  do 4![iSplit => //].
+  iDestruct "p_m2" as "[comp|p_m2]".
+  - iPoseProof (honest_frag_compromised_at with "honI comp")
+      as "%comp" => //.
+    rewrite /in_honest bool_decide_decide decide_False //.
+    tauto.
+  - iDestruct "p_m2"
+      as "(%b & %n' & %T' & %γ' & % & % & ? & ?)".
+    case: in_honest => //.
+    iExists b, n', T', γ'.
+    eauto. }
+case hon: (in_honest kI kR T); last first.
+{ iAssert (public a) as "{p_a} p_a".
+    by iApply "p_a".
   wp_pures. iApply ("Hpost" $! (Some (Spec.texp gb a))).
-  iFrame. iModIntro. iSplit; first by iApply public_minted.
-  iSplit => //. }
-iPoseProof (public_TEncE with "p_m2 [//]") as "[[contra _]|(#p & _ & _)]".
-{ iMod (honest_public with "[//] hon contra") as "H" => //.
-  - solve_ndisj.
-  - wp_pures. iDestruct "H" as ">[]". }
-iDestruct "p" as "(%ga & %b & %kI' & %n' & %T' & p)".
+  iFrame. iModIntro. iSplit; first by iApply minted_texp.
+  iSplit => //=.
+  iModIntro.
+  iSplit => //=; eauto.
+  iIntros "_". by iApply public_texp. }
+iDestruct "p_m2" as "[comp|p_m2]".
+{ rewrite /in_honest bool_decide_eq_true in hon.
+  iPoseProof (honest_frag_compromised_at with "honI comp") as "%" => //.
+  tauto. }
+rewrite /in_honest bool_decide_eq_true in hon.
+case: hon => honI honR.
+iDestruct "p_m2"
+  as "(%b & %n' & %T' & %γ' & -> & %n'_n & p_b & p_m2)".
+rewrite Spec.texpA.
 wp_pures.
-iDestruct "p" as "(%e & p_b & b_pred & honR & sessionR)".
-case/Spec.of_list_inj: e => <- -> <- {ga gb kI'}.
-rewrite !Spec.texpA.
-iPoseProof (honest_auth_frag_agree with "hon honR") as "[%n'n %agree]".
 iApply ("Hpost" $! (Some (TExp (TInt 0) [a; b]))). iFrame.
 rewrite !minted_TExp /= minted_TInt.
 iDestruct "m_gb" as "(_ & m_b & _)". iModIntro.
 iSplit; first do ![iSplit => //].
 iSplit => //.
-iSplit.
-{ iExists (TExp (TInt 0) [a]), b, n', T'.
-  rewrite Spec.texpA [TExp _ [a; b]]TExpC2. iSplit => //.
-  iSplit => //. }
+iModIntro.
 rewrite public_TExp2.
-iIntros "!> [[_ #p_b'] | [[_ p_a'] | (_ & a_pred' & _)]]".
+iSplit; last first.
+{ iIntros "#contra".
+  iRight. iLeft. iSplit => //. iApply "p_a". by eauto. }
+iIntros "[[_ #p_b'] | [[_ p_a'] | (_ & a_pred' & _)]]".
 - iPoseProof ("p_b" with "p_b'") as "{p_b} p_b".
   iModIntro. iDestruct "p_b" as "[#compR | #compI]".
-  + iPoseProof (honest_frag_compromised_at _ _ n'n with "honI compR") as "%".
+  + iPoseProof (honest_frag_compromised_at _ _ n'_n with "honI compR") as "%".
     set_solver.
-  + iPoseProof (honest_frag_compromised_at _ _ n'n with "honI compI") as "%".
+  + iPoseProof (honest_frag_compromised_at _ _ n'_n with "honI compI") as "%".
     set_solver.
 - iPoseProof ("p_a" with "p_a'") as ">%hon". tauto.
 - iPoseProof ("a_pred" with "a_pred'") as ">%contra".
   by have := contra _ _ eq_refl.
 Qed.
 
-Lemma wp_responder c kR dq n T E :
+Lemma wp_responder c kR dq n T γ E :
   ↑cryptisN ⊆ E →
   ↑N ⊆ E →
   channel c -∗
@@ -262,11 +305,8 @@ Lemma wp_responder c kR dq n T E :
         ⌜vkI = TKey Dec kI⌝ ∗
         minted kI ∗
         minted kS ∗
-        session kI kR kS Resp ∗
-        if in_honest kI kR T then
-          session kI kR kS Init ∗
-          □ (public kS -∗ ▷ False)
-        else public kS
+        session γ kI kR kS Resp (in_honest kI kR T) ∗
+        □ (public kS ↔ ▷ ⌜negb (in_honest kI kR T)⌝)
       else True
  }}}.
 Proof.
@@ -281,8 +321,8 @@ wp_bind (is_key _). iApply wp_is_key.
 case: Spec.is_keyP => [kt kI -> {vkI}|]; last by protocol_failure.
 wp_pures. case: kt => //=; first by protocol_failure.
 wp_pures. wp_bind (mknonce _).
-iApply (wp_mknonce (λ _, compromised_at n (TKey Enc kR) ∨
-                         compromised_at n (TKey Enc kI))%I dh_auth_pred).
+iApply (wp_mknonce (λ _, compromised_at n (TKey Enc kI) ∨
+                         compromised_at n (TKey Enc kR))%I dh_auth_pred).
 iIntros "%b #m_b #p_b #dh_gb token".
 iAssert (public (TExp (TInt 0) [b])) as "#p_gb".
 { iApply public_TExp1. rewrite minted_TInt.
@@ -292,9 +332,9 @@ iAssert (public (TExp (TInt 0) [b])) as "#p_gb".
   by rewrite -(Permutation_length perm). }
 wp_pure _ credit:"H1".
 wp_pure _ credit:"H2".
-wp_pures. wp_bind (mkkeyshare _). iApply wp_mkkeyshare => //.
+wp_bind (mkkeyshare _). iApply wp_mkkeyshare => //.
 iIntros "!> _". wp_pures. wp_list. wp_term_of_list. wp_tenc.
-iMod (term_meta_set _ _ (Resp, ga, b, kI, kR, n, T)
+iMod (term_meta_set _ _ (Resp, ga, kI, kR, n, T, γ)
        (N.@"session") with "token")
   as "#meta"; first solve_ndisj.
 iPoseProof (honest_auth_frag with "hon_auth") as "#honR".
@@ -303,7 +343,7 @@ wp_pures. wp_bind (send _ _). iApply wp_send => //.
   iApply public_TEncIS => //.
   - by rewrite public_minted !minted_TKey.
   - iModIntro.
-    iExists ga, b, kI, n, T.  by do 5![iSplitL => //].
+    iExists ga, b, kI, n, T, γ.  by do ![iSplitL => //].
   - rewrite minted_of_list /= minted_TExp minted_TInt /=.
     rewrite !public_minted !minted_TKey. by do ![iSplitL => //].
   - iIntros "!> _". rewrite public_of_list /=.
@@ -316,94 +356,93 @@ wp_list_match => [ga' gb' vkR' -> {m3}|]; last by protocol_failure.
 wp_eq_term e; last by protocol_failure. subst ga'.
 wp_eq_term e; last by protocol_failure. subst gb'.
 wp_eq_term e; last by protocol_failure. subst vkR'.
-wp_pures. wp_bind (texp _ _). iApply wp_texp. wp_pures.
-iAssert (session kI kR (Spec.texp ga b) Resp) as "sessionR".
-{ iExists _, _, n, T; eauto. }
+wp_pure _ credit:"H3".
+wp_bind (texp _ _). iApply wp_texp.
+wp_pure _ credit:"H4".
+iPoseProof (public_TEncE with "p_m3 [//]") as "{p_m3} p_m3".
+rewrite public_of_list /=.
+iAssert ( |={E}=> ●H{dq|n} T ∗
+  □ (
+  (compromised_at n (TKey Enc kI) ∨ compromised_at n (TKey Enc kR)) ∨
+  ∃ a γ',
+    ⌜ga = TExp (TInt 0) [a]⌝ ∗
+    (public a ↔ ▷ □ ⌜negb (in_honest kI kR T)⌝) ∗
+    (∀ t, dh_pred a t ↔ ▷ □ dh_auth_pred t) ∗
+    nonce_meta a (N.@"session") (Init, TExp (TInt 0) [b], kI, kR, n, T, γ')))%I
+  with "[hon_auth H3 H4]"
+  as "{p_m3} > [hon_auth #i_m3]".
+{ iDestruct "p_m3" as "[(p_skI & _) | (#i_m3 & _ & _)]".
+  { iMod (compromised_atI with "[//] H3 hon_auth p_skI")
+      as "[hon_auth #comp]" => //; try by solve_ndisj. }
+  iMod (lc_fupd_elim_later_pers with "H4 i_m3") as "{i_m3} #i_m3".
+  iDestruct "i_m3" as "(%a & %gb & %kR' & %n' & %T' & %γ' & %e_m3 &
+                        p_a & pred_a & honI & sessionI & i_m3)".
+  case/Spec.of_list_inj: e_m3 => -> <- <- {ga gb kR'}.
+  iDestruct "i_m3" as "[i_m3 | i_m3]".
+  { iMod (compromised_atI with "[//] H3 hon_auth i_m3")
+      as "[hon_auth #comp]" => //; try by solve_ndisj. }
+  iDestruct "i_m3" as "(%b' & %n'' & %T'' & %γ'' & %e_b & %n''_n' & i_m3)".
+  case/TExp_inj: e_b => _ /(Permutation_singleton_inj _ _) <- {b'}.
+  iPoseProof (term_meta_agree with "meta i_m3") as "%e_meta".
+  case: e_meta => <- <- <- {n'' T'' γ''} in n''_n' *.
+  iPoseProof (honest_auth_frag_agree with "hon_auth honI") as "[%n'_n %T'_T]".
+  rewrite -(T'_T n''_n') {T' T'_T}.
+  assert (n' = n) as -> by lia.
+  iModIntro. iFrame.
+  iRight. iModIntro. iExists a, γ'. by do ![iSplitL => //]. }
+iAssert (session γ kI kR (Spec.texp ga b) Resp (in_honest kI kR T))
+  as "sessionR".
+{ iExists _, _, n, T. iSplit => //.
+  do ![iSplit => //].
+  iDestruct "i_m3" as "[[comp | comp]|i_m3]".
+  - iPoseProof (honest_frag_compromised_at with "honR comp") as "%" => //.
+    rewrite /in_honest bool_decide_eq_false_2 //; tauto.
+  - iPoseProof (honest_frag_compromised_at with "honR comp") as "%" => //.
+    rewrite /in_honest bool_decide_eq_false_2 //; tauto.
+  case: in_honest => //.
+  iDestruct "i_m3" as "(%a & %γ' & -> & ? & ? & ?)".
+  iExists _, _, _, _; eauto. }
 iAssert (minted (Spec.texp ga b)) as "#m_kS".
 { iApply minted_texp => //. by iApply public_minted. }
 iAssert (minted kI) as "#m_kI".
 { iApply minted_TKey. by iApply public_minted. }
-iPoseProof (public_TEncE with "p_m3 [//]") as "{p_m3} p_m3".
-rewrite public_of_list /=.
-iAssert ( □ ▷ □ (
-  (public (TKey Enc kI) ∨ public (TKey Enc kR)) ∨
-  ∃ a,
-    ⌜ga = TExp (TInt 0) [a]⌝ ∗
-    (public a ↔ ▷ □ ⌜TKey Enc kI ∉ T ∨ TKey Enc kR ∉ T⌝) ∗
-    (∀ t, dh_pred a t ↔ ▷ □ dh_auth_pred t) ∗
-    nonce_meta a (N.@"session") (Init, TExp (TInt 0) [b], a, kI, kR, n, T)))%I
-  as "{p_m3} #i_m3".
-{ iDestruct "p_m3" as "[(p_skI & _) | (#i_m3 & _ & _)]";
-    first by iModIntro; eauto.
-  iApply bi.later_intuitionistically. iModIntro.
-  iDestruct "i_m3" as "(%a & %gb & %kR' & %n' & %T' & %e_m3 &
-                        p_a & pred_a & honI & sessionI & i_m3)".
-  case/Spec.of_list_inj: e_m3 => -> <- <- {ga gb kR'}.
-  iDestruct "i_m3" as "[i_m3 | i_m3]"; first by eauto.
-  iDestruct "i_m3" as "(%b' & %n'' & %T'' & %e_b & %n''_n' & i_m3)".
-  case/TExp_inj: e_b => _ /(Permutation_singleton_inj _ _) <- {b'}.
-  iPoseProof (term_meta_agree with "meta i_m3") as "%e_meta".
-  case: e_meta => <- <- {n'' T''} in n''_n' *.
-  iPoseProof (honest_auth_frag_agree with "hon_auth honI") as "[%n'_n %T'_T]".
-  rewrite -(T'_T n''_n') {T' T'_T}.
-  assert (n' = n) as -> by lia.
-  rewrite Spec.texpA TExpC2.
-  iModIntro. iModIntro.
-  iRight. iExists a. by do ![iSplitL => //]. }
-iMod (lc_fupd_elim_later with "H1 i_m3") as "{i_m3} #i_m3".
-iAssert (|={E}=> ●H{dq|n} T ∗ □ (
-  (compromised_at n (TKey Enc kR) ∨ compromised_at n (TKey Enc kI)) ∨
-  ∃ a,
-    ⌜ga = TExp (TInt 0) [a]⌝ ∗
-    (public a ↔ ▷ □ ⌜TKey Enc kI ∉ T ∨ TKey Enc kR ∉ T⌝) ∗
-    (∀ t, dh_pred a t ↔ ▷ □ dh_auth_pred t) ∗
-    nonce_meta a (N.@"session") (Init, TExp (TInt 0) [b], a, kI, kR, n, T)))%I
-  with "[hon_auth H2]" as "{i_m3} >[hon_auth #i_m3]".
-{ iDestruct "i_m3" as "[compromise|i_m3]"; last by iFrame; eauto.
-  iDestruct "compromise" as "[compromise|compromise]".
-  - iMod (compromised_atI with "[//] H2 hon_auth compromise")
-      as "[? #?]"; try solve_ndisj.
-  - iMod (compromised_atI with "[//] H2 hon_auth compromise")
-      as "[? #?]"; try solve_ndisj. }
 iDestruct "i_m3" as "[compromise|i_m3]".
-{ case: (decide (TKey Enc kI ∈ T ∧ TKey Enc kR ∈ T)) =>
-        [[honI honR]|compromise].
+{ iAssert (⌜in_honest kI kR T = false⌝)%I as "%hon".
   { iDestruct "compromise" as "[compI | compR]".
     - iPoseProof (honest_frag_compromised_at with "honR compI") as "%" => //.
-    - iPoseProof (honest_frag_compromised_at with "honR compR") as "%" => //. }
+      iPureIntro. apply/bool_decide_eq_false. tauto.
+    - iPoseProof (honest_frag_compromised_at with "honR compR") as "%" => //.
+      iPureIntro. apply/bool_decide_eq_false. tauto. }
+  wp_pures.
   iApply ("Hpost" $! (Some (TKey Dec kI, Spec.texp ga b))).
   iFrame. iModIntro. iExists kI.
-  rewrite /in_honest bool_decide_decide decide_False //.
+  rewrite hon.
   do 4![iSplit => //].
-  iApply public_texp => //.
-  by iApply "p_b". }
-iDestruct "i_m3" as "(%a & -> & p_a & pred_a & metaI)".
-rewrite Spec.texpA TExpC2.
+  iModIntro.
+  iSplit.
+  - by eauto.
+  - iIntros "/= #contra". iApply public_texp => //.
+    iApply "p_b". by eauto. }
+iDestruct "i_m3" as "(%a & %γ' & -> & p_a & pred_a & metaI)".
+rewrite Spec.texpA TExpC2. wp_pures.
 iApply ("Hpost" $! (Some (TKey Dec kI, TExp (TInt 0) [a; b]))).
 iFrame. iModIntro. iExists kI. do 2![iSplit => //].
 rewrite minted_TExp minted_TInt /=. iSplit; first by eauto.
 iSplit => //.
-case: (decide (TKey Enc kI ∈ T ∧ TKey Enc kR ∈ T)) =>
-        [[honI honR]|compromise]; last first.
-- rewrite /in_honest bool_decide_decide decide_False //.
-  rewrite not_and_r in compromise.
-  rewrite -(Spec.texpA _ [b] a).
-  iApply public_texp => //.
-  iApply "p_a". eauto.
-- rewrite /in_honest bool_decide_decide decide_True //.
-  iSplitL.
-  { iExists (TExp (TInt 0) [b]), a, n, T.
-    rewrite Spec.texpA. do 2![iSplit => //]. }
-  iIntros "!> #p_kS".
-  iDestruct (public_TExp2 with "p_kS")
-  as "[[_ p_b'] | [ [_ p_a'] | (_ & contra & _)]]".
-  + iPoseProof ("p_b" with "p_b'") as "[comp|comp]"; iModIntro.
+rewrite public_TExp2. iModIntro. iSplit.
+- iIntros "#p_kS".
+  iDestruct "p_kS" as "[[_ p_b'] | [ [_ p_a'] | (_ & contra & _)]]".
+  + iPoseProof ("p_b" with "p_b'") as "#[#comp|#comp]"; iModIntro.
     * iDestruct (honest_frag_compromised_at with "honR comp") as "%" => //.
+      rewrite /in_honest bool_decide_eq_false_2 //=. tauto.
     * iDestruct (honest_frag_compromised_at with "honR comp") as "%" => //.
-  + iPoseProof ("p_a" with "p_a'") as ">%compromised".
-    by case: compromised => [/(_ honI) | /(_ honR)].
+      rewrite /in_honest bool_decide_eq_false_2 //=. tauto.
+  + iPoseProof ("p_a" with "p_a'") as "{p_a} p_a".
+    iModIntro. by eauto.
   + iPoseProof ("pred_a" with "contra") as ">%contra".
     by have := contra _ _ eq_refl.
+- iIntros "#comp". iRight. iLeft. iSplit => //.
+  iApply "p_a". by eauto.
 Qed.
 
 End Verif.
